progress on semax

veric/semax.v
@@ -9,6 +9,7 @@ Require Import VST.veric.Clight_lemmas.
 Require Import VST.sepcomp.extspec.
 Require Import VST.sepcomp.step_lemmas.
 Require Import VST.veric.juicy_safety.
+Require Import VST.veric.external_state.
 Require Import VST.veric.juicy_extspec.
 Require Import VST.veric.tycontext.
 Require Import VST.veric.expr2.
@@ -18,21 +19,24 @@ Import Ctypes Clight_core.
 
 Local Open Scope nat_scope.
 
-Definition closed_wrt_modvars c (F: assert) : Prop :=
+Section mpred.
+
+Context `{!heapGS Σ} (Espec : OracleKind) `{!externalGS OK_ty Σ}.
+
+Definition closed_wrt_modvars c (F: environ -> mpred) : Prop :=
     closed_wrt_vars (modifiedvars c) F.
 
-Definition genv_symb_injective {F V} (ge: Genv.t F V) : extspec.injective_PTree block.
+Definition genv_symb_injective {F V} (ge: Genv.t F V) : extspec.injective_PTree Values.block.
 Proof.
 exists (Genv.genv_symb ge).
 hnf; intros.
 eapply Genv.genv_vars_inj; eauto.
 Defined.
 
-Definition jsafeN {Z} (Hspec : juicy_ext_spec Z) (ge: genv) :=
-  @jsafeN_ genv _ _ genv_symb_injective 
-               (cl_core_sem ge) Hspec ge.
+Definition jsafeN (ge: genv) :=
+  jsafe(genv_symb := genv_symb_injective) (cl_core_sem ge) OK_spec ge.
 
-Definition ext_compat {Z} (ora : Z) (w : rmap) :=
+(*Definition ext_compat (ora : Z) (w : rmap) :=
   joins (ghost_of w) (Some (ghost_PCM.ext_ref ora, NoneP) :: nil).
 
 Lemma ext_compat_unage : forall {Z} (ora : Z) w w', age w w' ->
@@ -49,87 +53,39 @@ Proof.
   unfold ext_compat; intros.
   apply rmap_order in H as (? & ? & ?).
   eapply join_sub_joins_trans; eauto.
-Qed.
+Qed.*)
 
 Inductive contx :=
 | Stuck
 | Cont: cont -> contx
 | Ret: option val -> cont -> contx.
 
-
-Definition assert_safe'_ 
-     (Espec : OracleKind)
-     (ge: genv) (f: function) (ve: env) (te: temp_env) (ctl: contx) (rho: environ) 
-     (w : rmap) :=
-       forall ora (jm:juicy_mem),
-       ext_compat ora w ->
-       rho = construct_rho (filter_genv ge) ve te ->
-       m_phi jm = w ->
-       forall (LW: level w > O),
+Definition assert_safe
+     (ge: genv) (E: coPset) (f: function) (ve: env) (te: temp_env) (ctl: contx) (rho: environ) : mpred :=
+       ∀ ora, (* ext_compat ora -> *)
+       ⌜rho = construct_rho (filter_genv ge) ve te⌝ →
        match ctl with
-       | Stuck => jm_fupd ora Ensembles.Full_set Ensembles.Full_set (fun _ => False) jm
+       | Stuck => False
        | Cont (Kseq s ctl') => 
-             jm_fupd ora Ensembles.Full_set Ensembles.Full_set (jsafeN (@OK_spec Espec) ge ora (State f s ctl' ve te)) jm
+             jsafeN ge E ora (State f s ctl' ve te)
        | Cont (Kloop1 body incr ctl') =>
-             jm_fupd ora Ensembles.Full_set Ensembles.Full_set (jsafeN (@OK_spec Espec) ge ora (State f Sskip (Kloop1 body incr ctl') ve te)) jm
+             jsafeN ge E ora (State f Sskip (Kloop1 body incr ctl') ve te)
        | Cont (Kloop2 body incr ctl') =>
-             jm_fupd ora Ensembles.Full_set Ensembles.Full_set (jsafeN (@OK_spec Espec) ge ora (State f (Sloop body incr) ctl' ve te)) jm
+             jsafeN ge E ora (State f (Sloop body incr) ctl' ve te)
        | Cont (Kcall id' f' ve' te' k') => 
-             jm_fupd ora Ensembles.Full_set Ensembles.Full_set (jsafeN (@OK_spec Espec) ge ora (State f (Sreturn None) (Kcall id' f' ve' te' k') ve te)) jm
+             jsafeN ge E ora (State f (Sreturn None) (Kcall id' f' ve' te' k') ve te)
        | Cont Kstop =>
-             jm_fupd ora Ensembles.Full_set Ensembles.Full_set (jsafeN (@OK_spec Espec) ge ora (State f (Sreturn None) Kstop ve te)) jm
-       | Cont _ => jm_fupd ora Ensembles.Full_set Ensembles.Full_set (fun _ => False) jm
+             jsafeN ge E ora (State f (Sreturn None) Kstop ve te)
+       | Cont _ => False
        | Ret None ctl' =>
-                jsafeN (@OK_spec Espec) ge ora (State f (Sreturn None) ctl' ve te) jm
-       | Ret (Some v) ctl' => forall e v',
-                  Clight.eval_expr ge ve te (m_dry jm) e v' ->
-                  Cop.sem_cast v' (typeof e) (fn_return f) (m_dry jm) = Some v ->
-              jsafeN (@OK_spec Espec) ge ora (State f (Sreturn (Some e)) ctl' ve te) jm
+                jsafeN ge E ora (State f (Sreturn None) ctl' ve te)
+       | Ret (Some v) ctl' => ∀ e v' m, coherent_with m →
+                  ⌜Clight.eval_expr ge ve te m e v'⌝ →
+                  ⌜Cop.sem_cast v' (typeof e) (fn_return f) m = Some v⌝ →
+              jsafeN ge E ora (State f (Sreturn (Some e)) ctl' ve te)
        end.
-(* upd in assert_safe'_, everywhere except ret? *)
 
-Notation fupd := (fupd Ensembles.Full_set Ensembles.Full_set).
-
-Program Definition assert_safe
-     (Espec : OracleKind) (ge: genv) (f: function) (ve: env) (te: temp_env) 
-     (ctl: contx) : assert :=
-  fun rho => assert_safe'_ (Espec : OracleKind) ge f ve te ctl rho.
-Next Obligation.
-  split; repeat intro.
-   subst.
-   destruct (oracle_unage _ _ H) as [jm0 [? ?]].
-   specialize (H0 ora jm0).
-   spec H0.
-   { eapply ext_compat_unage; eauto. }
-   specialize (H0 (eq_refl _) H3).
-   spec H0. apply age_level in H. lia.
-  subst.
-  destruct ctl; [|destruct c|]; try (eapply jm_fupd_age; eauto).
-  destruct o; intros; auto;
-  eapply age_safe; eauto.
-  rewrite (age_jm_dry H2) in *.
-  eapply H0; eauto.
-
-  subst. destruct (ext_ord_juicy_mem' _ _ H) as (? & Hd & Ha).
-  destruct (proj1 (rmap_order _ _) H) as (Hl & Hr & Hg).
-  destruct (juicy_mem_resource jm a) as (jm0 & Hjm & Hdry).
-  { congruence. }
-  specialize (H0 ora jm0).
-   spec H0.
-   { eapply ext_compat_unext; eauto. }
-   specialize (H0 (eq_refl _) Hjm).
-   spec H0. rewrite Hl; auto.
-  subst.
-  rewrite <- Hjm in *.
-  assert (ext_order jm0 jm) by (split; auto; congruence).
-  destruct ctl; [|destruct c|];
-    try (eapply jm_fupd_ext; eauto; intros; eapply ext_safe; eauto).
-  destruct o; intros; auto;
-  eapply ext_safe; eauto.
-  rewrite Hdry in *; eapply H0; eauto.
-Qed.
-
-Lemma assert_safe_derives : forall (Espec : OracleKind) (ge ge': genv) (f f': function) (ve ve': env) (te te': temp_env)
+(*Lemma assert_safe_derives : forall (Espec : OracleKind) (ge ge': genv) (f f': function) (ve ve': env) (te te': temp_env)
      (ctl ctl': contx) rho rho',
   (forall w ora (jm:juicy_mem),
        ext_compat ora w ->
@@ -181,7 +137,7 @@ Proof.
   repeat intro.
   edestruct H as [? Hsafe]; eauto.
   apply Hsafe, H0; auto.
-Qed.
+Qed.*)
 
 Definition list2opt {T: Type} (vl: list T) : option T :=
  match vl with nil => None | x::_ => Some x end.
@@ -199,17 +155,17 @@ Lemma guard_environ_e1:
      typecheck_environ Delta rho.
 Proof. intros. destruct H; auto. Qed.
 
-Definition _guard (Espec : OracleKind)
-    (gx: genv) (Delta: tycontext) (f: function) (P : assert) (ctl: contx) : pred nat :=
-     ALL tx : Clight.temp_env, ALL vx : env,
+Definition _guard
+    (gx: genv) E (Delta: tycontext) (f: function) (P : environ -> mpred) (ctl: contx) : mpred :=
+     ∀ tx : Clight.temp_env, ∀ vx : env,
           let rho := construct_rho (filter_genv gx) vx tx in
-          !! guard_environ Delta f rho
-                  && P rho && funassert Delta rho
-             >=> assert_safe Espec gx f vx tx ctl rho.
+          ■ ⌜guard_environ Delta f rho⌝
+                  ∧ P rho ∧ funassert Delta rho
+             -∗ assert_safe gx E f vx tx ctl rho.
 
-Definition guard (Espec : OracleKind)
-    (gx: genv) (Delta: tycontext) f (P : assert)  (ctl: cont) : pred nat :=
-  _guard Espec gx Delta f P (Cont ctl).
+Definition guard'
+    (gx: genv) E (Delta: tycontext) f (P : assert)  (ctl: cont) :=
+  _guard gx E Delta f P (Cont ctl).
 
 Fixpoint break_cont (k: cont) :=
 match k with
@@ -237,40 +193,17 @@ Definition exit_cont (ek: exitkind) (vl: option val) (k: cont) : contx :=
   end.
 
 Definition rguard (Espec : OracleKind)
-    (gx: genv) (Delta: tycontext) (f: function) (R : ret_assert) (ctl: cont) : pred nat :=
-  ALL ek: exitkind, ALL vl: option val,
-    _guard Espec gx Delta f (proj_ret_assert R ek vl)  (exit_cont ek vl ctl).
+    (gx: genv) E (Delta: tycontext) (f: function) (R : ret_assert) (ctl: cont) : mpred :=
+  ∀ ek: exitkind, ∀ vl: option val,
+    _guard gx E Delta f (proj_ret_assert R ek vl)  (exit_cont ek vl ctl).
 
 Record semaxArg :Type := SemaxArg {
  sa_cs: compspecs;
  sa_Delta: tycontext;
- sa_P: assert;
+ sa_P: environ -> mpred;
  sa_c: statement;
  sa_R: ret_assert
 }.
-
-Program Definition ext_spec_pre' (Espec: OracleKind) (ef: external_function)
-   (x': ext_spec_type OK_spec ef) (ge_s: injective_PTree block)
-   (ts: list typ) (args: list val) (z: OK_ty) : pred juicy_mem :=
-  fun jm => ext_compat z (m_phi jm) -> ext_spec_pre OK_spec ef x' ge_s ts args z jm.
-Next Obligation.
-Proof.
-  split; repeat intro.
-  - eapply ext_compat_unage in H1; [|eapply age_jm_phi; eauto].
-    eapply JE_pre_hered; eauto.
-  - eapply JE_pre_ext, H0; auto.
-    destruct H; eapply ext_compat_unext; eauto.
-Qed.
-
-Program Definition ext_spec_post' (Espec: OracleKind)
-   (ef: external_function) (x': ext_spec_type OK_spec ef) (ge_s: injective_PTree block)
-   (tret: rettype) (ret: option val) (z: OK_ty) : pred juicy_mem :=
-  exist (fun p => hereditary age p /\ hereditary ext_order p)
-   (ext_spec_post OK_spec ef x' ge_s tret ret z)
-     (conj (JE_post_hered _ _ _ _ _ _ _ _) (JE_post_ext _ _ _ _ _ _ _ _) ).
-
-(*Definition juicy_mem_pred (P : pred rmap) (jm: juicy_mem): pred nat :=
-     # diamond fashionM (exactly (m_phi jm) && P).*)
 
 Definition make_ext_rval  (gx: genviron) (tret: rettype) (v: option val):=
   match tret with AST.Tvoid => mkEnviron gx (Map.empty _) (Map.empty _) 
@@ -281,40 +214,27 @@ Definition make_ext_rval  (gx: genviron) (tret: rettype) (v: option val):=
   | None => mkEnviron gx (Map.empty _) (Map.empty _)
   end end.
 
-(*Program Definition if_ext_compat {Z} (z : Z) (P : pred juicy_mem) : pred juicy_mem :=
-  fun jm => ext_compat z (m_phi jm) -> P jm.
-Next Obligation.
-Proof.
-  unfold ext_compat; split; repeat intro.
-  - eapply pred_hereditary, H0; auto.
-    erewrite age1_ghost_of in H1 by (apply age1_juicy_mem_Some; eauto).
-    apply ext_join_unapprox in H1; auto.
-  - eapply pred_upclosed, H0; auto.
-    rewrite rmap_order in H; destruct H as (_ & _ & _ & ?).
-    eapply join_sub_joins_trans; eauto.
-Qed.*)
-
+(* Should this and funspec_sub both be indexed by a mask? *)
 Definition semax_external
-  (Hspec: OracleKind) ef
-  (A: TypeTree)
-  (P: forall ts, dependent_type_functor_rec ts (ArgsTT A) mpred)
-  (Q: forall ts, dependent_type_functor_rec ts (AssertTT A) mpred):
-        pred nat :=
- ALL gx: genv, ALL Ts: list Type,
- ALL x: (dependent_type_functor_rec Ts A (pred rmap)),
-   |>  ALL F: pred rmap, ALL ts: list typ,
-   ALL args: list val,
-   !!Val.has_type_list args (sig_args (ef_sig ef)) &&
-   juicy_mem_op (P Ts x (filter_genv gx, args) * F) >=>
-   EX x': ext_spec_type OK_spec ef,
-    (ALL z:_, ext_spec_pre' Hspec ef x' (genv_symb_injective gx) ts args z) &&
-     ! ALL tret: rettype, ALL ret: option val, ALL z': OK_ty,
-      ext_spec_post' Hspec ef x' (genv_symb_injective gx) tret ret z' >=>
-          juicy_mem_op (Q Ts x (make_ext_rval (filter_genv gx) tret ret) * F).
+  ef
+  (A: Type)
+  (P: A -> argsEnviron -> mpred)
+  (Q: A -> environ -> mpred) :=
+ ∀ gx: genv,
+ ∀ x: A,
+   ▷ ∀ F (ts: list typ),
+   ∀ args: list val,
+   ■ (⌜Val.has_type_list args (sig_args (ef_sig ef))⌝ ∧
+     ⎡P x (filter_genv gx, args) ∗ F⎤ ={⊤}=∗
+   ∃ x': ext_spec_type OK_spec ef,
+    (∀ z:_, ext_jmpred_pre OK_ty OK_spec ef x' (genv_symb_injective gx) ts args z) ∧
+     □ ∀ tret: rettype, ∀ ret: option val, ∀ z': OK_ty,
+      ext_jmpred_post OK_ty OK_spec ef x' (genv_symb_injective gx) tret ret z' ={⊤}=∗
+          ⎡Q x (make_ext_rval (filter_genv gx) tret ret) ∗ F⎤).
 
 Lemma Forall2_implication {A B} (P Q:A -> B -> Prop) (PQ:forall a b, P a b -> Q a b):
   forall l t, Forall2 P l t -> Forall2 Q l t.
-Proof. intros. induction H; constructor; auto. Qed.
+Proof. intros; eapply Forall2_impl; eauto. Qed.
 Lemma has_type_list_Forall2: forall vals ts, Val.has_type_list vals ts <-> Forall2 Val.has_type vals ts.
 Proof.
   induction vals; destruct ts; simpl; split; intros; trivial; try contradiction.
@@ -324,63 +244,35 @@ Proof.
 Qed.
 
 Lemma semax_external_funspec_sub
-  (DISABLE: False)
-  {Espec argtypes rtype cc ef A1 P1 Q1 P1ne Q1ne A P Q Pne Qne}
-  (Hsub: funspec_sub (mk_funspec (argtypes, rtype) cc A1 P1 Q1 P1ne Q1ne) 
-                     (mk_funspec (argtypes, rtype) cc A P Q Pne Qne))
+  {argtypes rtype cc ef A1 P1 Q1 A P Q}
+  (Hsub: funspec_sub (mk_funspec (argtypes, rtype) cc A1 P1 Q1)
+                     (mk_funspec (argtypes, rtype) cc A P Q))
   (HSIG: ef_sig ef = 
          mksignature
                      (map typ_of_type argtypes)
                      (rettype_of_type rtype) cc):
-  @semax.semax_external Espec ef A1 P1 Q1 |-- @semax.semax_external Espec ef A P Q.
-  (* This needs a fupd, but it's unclear how, since it's a pred nat. *)
+  semax_external ef A1 P1 Q1 ⊢ semax_external ef A P Q.
 Proof.
-apply allp_derives; intros g.
-apply allp_right; intros ts.
-apply allp_right; intros x.
-destruct Hsub as [_ H]; simpl in H.
-intros n N m NM F typs vals y MY ? z YZ EZ [HT HP].
-simpl in HP.
-rewrite HSIG in HT; simpl in HT.
-eapply sepcon_derives, fupd_frame_r in HP; [| intros ??; eapply H; split; eauto | apply derives_refl].
-2: { clear -HT. 
-  apply has_type_list_Forall2 in HT.
-  eapply Forall2_implication; [ | apply HT]; auto.
-}
-clear H. (*
-edestruct HP as (? & ? & z0 & ? & ? & ? & H); subst.
-{ eexists. rewrite ghost_fmap_core. apply join_comm, core_unit. }
-destruct H as [z1 [z2 [JZ [[ts1 [x1 [FRM [[z11 [z12 [JZ1 [H_FRM H_P1]]]] HQ]]]] Z2]]]].
-specialize (N ts1 x1). apply join_comm in JZ1.
-destruct (join_assoc JZ1 JZ) as [zz [JJ JJzz]]. apply join_comm in JJ.
-destruct (juicy_mem_resource _ _ H2) as (jm0 & ? & ?); subst.
-edestruct (N _ NM (sepcon F FRM) typs vals jm0) as [est [EST1 EST2]]; clear N; eauto.
-{ apply necR_level in YZ. destruct EZ as [_ EZ%ext_level]. rewrite !level_juice_level_phi in *. lia. }
-{ rewrite HSIG; simpl. split; trivial.
-  exists z12, zz; split3. trivial. trivial.
-  exists z2, z11; split3; trivial. }
-exists est; split.
-{ simpl. intros. apply EST1; auto. apply necR_trans with z; auto.*)
-contradiction DISABLE.  (* 
-    This lemma is not true as written because it needs a ghost-state
-    update operator somewhere.  
-*)
-  (*rewrite age_to.necR_age_to_iff. admit.
-simpl; intros.
-destruct (EST2 b b0 b1 _ H _ H0 H1) as [u1 [u2 [JU [U1 U2]]]]; clear EST2.
-destruct U2 as [w1 [w2 [JW [W1 W2]]]]. apply join_comm in JU.
-destruct (join_assoc JW JU) as [v [JV V]]. apply join_comm in V.
-exists v, w1; split3; trivial.
-apply HQ; clear HQ; split.
-+ simpl. destruct b,b0; reflexivity.
-+ exists w2, u1; split3; trivial.*)
+  apply bi.forall_mono; intros g.
+  iIntros "#H" (x). iIntros "!>" (F ts args) "!> (%HT & P & F)".
+  destruct Hsub as [[??] Hsub]; subst.
+  iMod (Hsub with "[$P]") as (x1 F1) "((F1 & P1) & %HQ)".
+  { iPureIntro; split; auto.
+    rewrite HSIG in HT; apply has_type_list_Forall2 in HT.
+    eapply Forall2_implication; [ | apply HT]; auto. }
+  iMod ("H" $! _ (F ∗ F1) with "[$P1 $F $F1]") as (x') "[Hpre #HQ1]"; first done.
+  iExists x'; iFrame.
+  iIntros "!> !>" (???) "Hpost".
+  iMod ("HQ1" with "Hpost") as "(Q1 & $ & F1)".
+  iApply (HQ with "[$F1 $Q1]"); iPureIntro; split; auto.
+  destruct tret, ret; auto.
 Qed.
 
 Definition tc_option_val (sig: type) (ret: option val) :=
   match sig, ret with
-    | Tvoid, _ => True
+    | Tvoid, _ => True%type
     | ty, Some v => tc_val ty v
-    | _, _ => False
+    | _, _ => False%type
   end.
 
 Fixpoint zip_with_tl {A : Type} (l1 : list A) (l2 : typelist) : list (A*type) :=
@@ -389,48 +281,42 @@ Fixpoint zip_with_tl {A : Type} (l1 : list A) (l2 : typelist) : list (A*type) :=
     | _, _ => nil
   end.
 
-Definition withtype_empty (A: TypeTree) : Prop :=
-  forall ts (x: dependent_type_functor_rec ts A (pred rmap)), False.
-Definition believe_external (Hspec: OracleKind) (gx: genv) (v: val) (fsig: typesig) cc
-  (A: TypeTree)
-  (P: forall ts, dependent_type_functor_rec ts (ArgsTT A) mpred)
-  (Q: forall ts, dependent_type_functor_rec ts (AssertTT A) mpred):
-  pred nat :=
+Definition withtype_empty (A: Type) : Prop := forall (x : A), False.
+Definition believe_external (gx: genv) (v: val) (fsig: typesig) cc
+  (A: Type)
+  (P: A -> argsEnviron -> mpred)
+  (Q: A -> environ -> mpred) :=
   match Genv.find_funct gx v with
   | Some (External ef sigargs sigret cc') =>
-        !! (fsig = (typelist2list sigargs, sigret) /\ cc'=cc
+        ⌜fsig = (typelist2list sigargs, sigret) /\ cc'=cc
            /\ ef_sig ef = mksignature
                            (typlist_of_typelist (typelist_of_type_list (fst fsig)))
                            (rettype_of_type (snd fsig)) cc
-           /\ (ef_inline ef = false \/ withtype_empty A))
-        && semax_external Hspec ef A P Q
-        && ! (ALL ts: list Type,
-              ALL x: dependent_type_functor_rec ts A (pred rmap),
-              ALL ret:option val,
-                Q ts x (make_ext_rval (filter_genv gx) (rettype_of_type (snd fsig)) ret)
-                  && !!Builtins0.val_opt_has_rettype ret (rettype_of_type (snd fsig))
-                  >=> !! tc_option_val sigret ret)
-  | _ => FF
+           /\ (ef_inline ef = false \/ withtype_empty A)⌝
+        ∧ semax_external ef A P Q
+        ∧ ■ (∀ x: A,
+              ∀ ret:option val,
+                ⎡Q x (make_ext_rval (filter_genv gx) (rettype_of_type (snd fsig)) ret)⎤
+                  ∧ ⌜Builtins0.val_opt_has_rettype ret (rettype_of_type (snd fsig))⌝
+                  -∗ ⌜tc_option_val sigret ret⌝)
+  | _ => False
   end.
 
-Lemma believe_external_funspec_sub {Espec gx v sig cc A P Q Pne Qne A' P' Q' Pne' Qne'}
-      (Hsub: funspec_sub (mk_funspec sig cc A P Q Pne Qne)(mk_funspec sig cc A' P' Q' Pne' Qne') )
+Lemma believe_external_funspec_sub {gx v sig cc A P Q A' P' Q'}
+      (Hsub: funspec_sub (mk_funspec sig cc A P Q)(mk_funspec sig cc A' P' Q') )
       (WTE: withtype_empty A -> withtype_empty A'):
-      believe_external Espec gx v sig cc A P Q |-- believe_external Espec gx v sig cc A' P' Q'.
+      believe_external gx v sig cc A P Q ⊢ believe_external gx v sig cc A' P' Q'.
 Proof.
-  unfold believe_external; intros n N.
+  unfold believe_external.
   destruct (Genv.find_funct gx v); trivial.
   destruct f; trivial. destruct sig as [argtypes rtype].
-  destruct N as [[[N1a [N1b [N1c N1d]]] N2] N3].
-  inv N1a. simpl in N1c; rewrite TTL2 in *; split.
-+ split.
-  - split3; trivial. split; trivial.
-    destruct N1d; [ left; trivial | right; auto].
-  - eapply semax_external_funspec_sub; try eassumption.
-     admit.
-+ simpl; intros. simpl in N3. simpl in Hsub.
-  destruct Hsub as [_ Hsub].
-  specialize (Hsub b b0).
+  iIntros "((% & % & %He & %) & H & #?)".
+  rewrite TTL2 in He |- *.
+  rewrite semax_external_funspec_sub; [iFrame | eauto..].
+  iSplit.
+  - iPureIntro; repeat split; auto; tauto.
+  - iIntros "!>" (??) "[Q %]".
+    destruct Hsub as [_ Hsub].
 Abort.
 
 Definition fn_funsig (f: function) : funsig := (fn_params f, fn_return f).
@@ -439,39 +325,39 @@ Definition var_sizes_ok (cenv: composite_env) (vars: list (ident*type)) :=
    Forall (fun var : ident * type => @sizeof cenv (snd var) <= Ptrofs.max_unsigned)%Z vars.
 
 Definition var_block' (sh: Share.t) (cenv: composite_env) (idt: ident * type) (rho: environ): mpred :=
-  !! (sizeof (snd idt) <= Ptrofs.max_unsigned)%Z &&
+  ⌜(sizeof (snd idt) <= Ptrofs.max_unsigned)%Z⌝ ∧
   (memory_block sh (sizeof (snd idt))) (eval_lvar (fst idt) (snd idt) rho).
 
-Definition stackframe_of' (cenv: composite_env) (f: Clight.function) : assert :=
-  fold_right (fun P Q rho => P rho * Q rho) (fun rho => emp)
+Definition stackframe_of' (cenv: composite_env) (f: Clight.function) : environ -> mpred :=
+  fold_right (fun P Q rho => P rho ∗ Q rho) (fun rho => emp)
      (map (fun idt => var_block' Share.top cenv idt) (Clight.fn_vars f)).
 
 Definition believe_internal_ CS
-  (semax:semaxArg -> pred nat)
-  (gx: genv) (Delta: tycontext) v (fsig: typesig) cc (A: TypeTree)
-  (P: forall ts, dependent_type_functor_rec ts (ArgsTT A) mpred)
-  (Q: forall ts, dependent_type_functor_rec ts (AssertTT A) mpred) : pred nat :=
+  (semax:semaxArg -> mpred)
+  (gx: genv) (Delta: tycontext) v (fsig: typesig) cc (A: Type)
+  (P: A -> argsEnviron -> mpred)
+  (Q: A -> environ -> mpred) :=
   let ce := (@cenv_cs CS) in
-  (EX b: block, EX f: function,
+  (∃ b: block, ∃ f: function,
    let specparams := fst fsig in 
    let fparams := fn_params f in
-   prop (v = Vptr b Ptrofs.zero /\ Genv.find_funct_ptr gx b = Some (Internal f)
+   ⌜v = Vptr b Ptrofs.zero /\ Genv.find_funct_ptr gx b = Some (Internal f)
                  /\ Forall (fun it => complete_type ce (snd it) = true) (fn_vars f)
                  /\ list_norepet (map fst fparams ++ map fst f.(fn_temps))
                  /\ list_norepet (map fst f.(fn_vars)) /\ var_sizes_ok ce (f.(fn_vars))
                  /\ specparams = map snd fparams
                  /\ snd fsig = snd (fn_funsig f)
-                 /\ f.(fn_callconv) = cc)
-  &&
-   ALL Delta':tycontext, ALL CS':compspecs,
+                 /\ f.(fn_callconv) = cc⌝
+  ∧
+   ∀ Delta':tycontext, ∀ CS':compspecs,
    imp (prop (forall f, tycontext_sub (func_tycontext' f Delta) (func_tycontext' f Delta')))
      (imp (prop (cenv_sub (@cenv_cs CS) (@cenv_cs CS'))) 
-      (ALL ts: list Type,
-       ALL x : dependent_type_functor_rec ts A (pred rmap),
-        |> semax (SemaxArg CS' (func_tycontext' f Delta')
+      (∀ ts: list Type,
+       ∀ x : dependent_type_functor_rec ts A (pred rmap),
+        ▷ semax (SemaxArg CS' (func_tycontext' f Delta')
                          (fun rho => (bind_args (f.(fn_params)) (P ts x) rho 
                                               * stackframe_of' (@cenv_cs CS') f rho)
-                                        && funassert (func_tycontext' f Delta') rho)
+                                        ∧ funassert (func_tycontext' f Delta') rho)
                           (f.(fn_body))
            (frame_ret_assert (function_body_ret_assert (fn_return f) (Q ts x)) 
               (stackframe_of' (@cenv_cs CS') f)))) )).
@@ -484,10 +370,10 @@ Definition claims (ge: genv) (Delta: tycontext) v fsig cc A P Q : Prop :=
 
 Definition believepred CS (Espec: OracleKind) (semax: semaxArg -> pred nat)
               (Delta: tycontext) (gx: genv)  (Delta': tycontext) : pred nat :=
-  ALL v:val, ALL fsig: typesig, ALL cc: calling_convention,
-  ALL A: TypeTree,
-  ALL P: forall ts, dependent_type_functor_rec ts (ArgsTT A) mpred,
-  ALL Q: forall ts, dependent_type_functor_rec ts (AssertTT A) mpred,
+  ∀ v:val, ∀ fsig: typesig, ∀ cc: calling_convention,
+  ∀ A: TypeTree,
+  ∀ P: forall ts, dependent_type_functor_rec ts (ArgsTT A) mpred,
+  ∀ Q: forall ts, dependent_type_functor_rec ts (AssertTT A) mpred,
        !! claims gx Delta' v fsig cc A P Q  -->
       (believe_external Espec gx v fsig cc A P Q
         || believe_internal_ CS semax gx Delta v fsig cc A P Q).
@@ -495,13 +381,13 @@ Definition believepred CS (Espec: OracleKind) (semax: semaxArg -> pred nat)
 Definition semax_ (Espec: OracleKind)
        (semax: semaxArg -> pred nat) (a: semaxArg) : pred nat :=
  match a with SemaxArg CS Delta P c R =>
-  ALL gx: genv, ALL Delta': tycontext,ALL CS':compspecs,
+  ∀ gx: genv, ∀ Delta': tycontext,∀ CS':compspecs,
        !! (tycontext_sub Delta Delta' 
             /\ cenv_sub (@cenv_cs CS) (@cenv_cs CS') 
             /\ cenv_sub (@cenv_cs CS') (genv_cenv gx)) -->
       (believepred CS' Espec semax Delta' gx Delta') -->
-     ALL k: cont, ALL F: assert, ALL f:function,
-       (!! (closed_wrt_modvars c F) &&
+     ∀ k: cont, ∀ F: assert, ∀ f:function,
+       (!! (closed_wrt_modvars c F) ∧
               rguard Espec gx Delta' f (frame_ret_assert R F) k) -->
         guard Espec gx Delta' f (fun rho => F rho * P rho) (Kseq c k)
   end.
@@ -514,7 +400,7 @@ Definition believe_internal {CS: compspecs} (Espec:  OracleKind)
   (P: forall ts, dependent_type_functor_rec ts (ArgsTT A) mpred)
   (Q: forall ts, dependent_type_functor_rec ts (AssertTT A) mpred): pred nat :=
   let ce := @cenv_cs CS in
-  (EX b: block, EX f: function,
+  (∃ b: block, ∃ f: function,
    let specparams := fst fsig in 
    let fparams := fn_params f in
    prop (v = Vptr b Ptrofs.zero /\ Genv.find_funct_ptr gx b = Some (Internal f)
@@ -524,37 +410,37 @@ Definition believe_internal {CS: compspecs} (Espec:  OracleKind)
                  /\ specparams = map snd fparams
                  /\ snd fsig = snd (fn_funsig f)
                  /\ f.(fn_callconv) = cc)
-  && 
-    ALL Delta':tycontext,ALL CS':compspecs,
+  ∧ 
+    ∀ Delta':tycontext,∀ CS':compspecs,
      imp (prop (forall f, tycontext_sub (func_tycontext' f Delta) (func_tycontext' f Delta')))
       (imp (prop (cenv_sub (@cenv_cs CS) (@cenv_cs CS')))
-       (ALL ts: list Type,
-     ALL x : dependent_type_functor_rec ts A (pred rmap),
-     |> @semax' CS' Espec (func_tycontext' f Delta')
+       (∀ ts: list Type,
+     ∀ x : dependent_type_functor_rec ts A (pred rmap),
+     ▷ @semax' CS' Espec (func_tycontext' f Delta')
                                 (fun rho => (bind_args (f.(fn_params)) (P ts x) rho * stackframe_of' (@cenv_cs CS') f rho)
-                                             && funassert (func_tycontext' f Delta') rho)
+                                             ∧ funassert (func_tycontext' f Delta') rho)
                                (f.(fn_body))
            (frame_ret_assert (function_body_ret_assert (fn_return f) (Q ts x)) (stackframe_of' (@cenv_cs CS') f))))).
 
 Definition believe {CS: compspecs} (Espec:OracleKind)
               (Delta: tycontext) (gx: genv) (Delta': tycontext): pred nat :=
-  ALL v:val, ALL fsig: typesig, ALL cc: calling_convention,
-  ALL A: TypeTree,
-  ALL P: (forall ts, dependent_type_functor_rec ts (ArgsTT A) (pred rmap)),
-  ALL Q: (forall ts, dependent_type_functor_rec ts (AssertTT A) (pred rmap)),
+  ∀ v:val, ∀ fsig: typesig, ∀ cc: calling_convention,
+  ∀ A: TypeTree,
+  ∀ P: (forall ts, dependent_type_functor_rec ts (ArgsTT A) (pred rmap)),
+  ∀ Q: (forall ts, dependent_type_functor_rec ts (AssertTT A) (pred rmap)),
        !! claims gx Delta' v fsig cc A P Q  -->
       (believe_external Espec gx v fsig cc A P Q
         || believe_internal Espec gx Delta v fsig cc A P Q).
 
 Lemma semax_fold_unfold : forall {CS: compspecs} (Espec : OracleKind),
   semax' Espec = fun Delta P c R =>
-  ALL gx: genv, ALL Delta': tycontext,ALL CS':compspecs,
+  ∀ gx: genv, ∀ Delta': tycontext,∀ CS':compspecs,
        !! (tycontext_sub Delta Delta'
            /\ cenv_sub (@cenv_cs CS) (@cenv_cs CS')
            /\ cenv_sub (@cenv_cs CS') (genv_cenv gx)) -->
        @believe CS' Espec Delta' gx Delta' -->
-     ALL k: cont, ALL F: assert, ALL f: function,
-        (!! (closed_wrt_modvars c F) && rguard Espec gx Delta' f (frame_ret_assert R F) k) -->
+     ∀ k: cont, ∀ F: assert, ∀ f: function,
+        (!! (closed_wrt_modvars c F) ∧ rguard Espec gx Delta' f (frame_ret_assert R F) k) -->
         guard Espec gx Delta' f (fun rho => F rho * P rho) (Kseq c k).
 Proof.
 intros ? ?.
@@ -622,7 +508,7 @@ Qed.
 
 Lemma allp_andp: 
   forall {A} {NA: ageable A} {EO: Ext_ord A} {B: Type} (b0: B) (P: B -> pred A) (Q: pred A),
-   (allp P && Q = allp (fun x => P x && Q))%pred.
+   (allp P ∧ Q = allp (fun x => P x ∧ Q))%pred.
 Proof.
 intros.
 apply pred_ext.
@@ -676,7 +562,7 @@ Qed.
 
 Lemma andp_imp_e':
   forall (A : Type) (agA : ageable A) (EO: Ext_ord A) (P Q : pred A),
-   P && (P --> Q) |-- P && Q.
+   P ∧ (P --> Q) |-- P ∧ Q.
 Proof.
 intros.
 apply andp_right.
@@ -699,7 +585,7 @@ Qed.
 
 Lemma imp_imp:
   forall (A : Type) (agA : ageable A) (EO : Ext_ord A) (P Q R: pred A),
-    P --> (Q --> R) = P && Q --> R.
+    P --> (Q --> R) = P ∧ Q --> R.
 Proof.
   intros.
   apply pred_ext.
@@ -717,7 +603,7 @@ Qed.
 
 Lemma imp_allp:
   forall B (A : Type) (agA : ageable A) (EO : Ext_ord A) (P: pred A) (Q: B -> pred A),
-    P --> allp Q  = ALL x: B, P --> Q x.
+    P --> allp Q  = ∀ x: B, P --> Q x.
 Proof.
   intros.
   apply pred_ext.
@@ -941,3 +827,5 @@ Lemma semax_cssub {CS CS'} (CSUB: cspecs_sub  CS CS') Espec Delta P c R:
 Proof.
   intros. intros n. apply (semax'_cssub CSUB); trivial. 
 Qed.
+
+End mpred.
